

Př~1:
\begin{align}
y'''+3y''+y' & = 2u'+3u \\
p^3Y(p)+ p^23Y(p)+ Y(p) & = 2p^2U(p)+3U(p) \\
Y(p)(p^3+p^2+1) & = U(p)(2p^2+3) \\
\frac{Y(p)}{U(p)} & = \frac{2p^2+3}{p^3+3p^2+1} \\
G(p) & = \frac{2p^2 + 3} { p^3 + 3p^2 + p}
\end{align}

Př~2:
\begin{align}
3y''''+2y''+5y'+2y & = 4~u'''+6u''+u \\
G(p) & = \frac{4p^3+6p^2+1}{3p^4+2p^2+5p+2} \\
\end{align}

Př~3: (A) \ref{eq:1}
\begin{equation} \label{eq:1}
\begin{aligned}
y'''+7y''+6y' & = u'+3u \\
G(s) & = \frac{s+3}{s^3+7s^2+6s} \\
G(s) & = \frac{s+3}{s(s+1)(s+6)} \\
G(s) & = \frac12 \frac{\frac13 s~+ 1}{s (\frac16 s~+ 1) (s + 1)}
\end{aligned}
\end{equation}

Př~4: (B) \ref{eq:2}
\begin{align} \label{eq:2}
y'' + 6y'+8y &= u''+4u'+3u \\
G(s) & = \frac{s^2 + 4s~+ 3}{s^2+6s+8} \\
G(s) & = \frac{(s+1)(s+3)}{(s+2)(s+4)} \\
G(s) & = \frac{3(s+1)(\frac13 s~+ 1)}{8(\frac12 s+1)(\frac14 s+1)}
\end{align}
